notations.lean
@@ -931,6 +931,138 @@ def propctx.apply: propctx → term → prop
 
 instance : has_coe_to_fun propctx := ⟨λ _, term → prop, propctx.apply⟩
 
+lemma unchanged_of_apply_termctx_without_hole {t tt: term}:
+      t.to_termctx tt = t :=
+  begin
+    induction t with v y unop t₁ ih₁ binop t₂ t₃ ih₂ ih₃ t₄ t₅ ih₄ ih₅,
+
+    show (termctx.apply (term.to_termctx (term.value v)) tt = term.value v), by begin
+      unfold term.to_termctx,
+      unfold termctx.apply
+    end,
+
+    show (termctx.apply (term.to_termctx (term.var y)) tt = term.var y), by begin
+      unfold term.to_termctx,
+      unfold termctx.apply
+    end,
+
+    show (termctx.apply (term.to_termctx (term.unop unop t₁)) tt = term.unop unop t₁), by begin
+      unfold term.to_termctx,
+      unfold termctx.apply,
+      congr,
+      from ih₁
+    end,
+
+    show (termctx.apply (term.to_termctx (term.binop binop t₂ t₃)) tt = term.binop binop t₂ t₃), by begin
+      unfold term.to_termctx,
+      unfold termctx.apply,
+      congr,
+      from ih₂,
+      from ih₃
+    end,
+
+    show (termctx.apply (term.to_termctx (term.app t₄ t₅)) tt = term.app t₄ t₅), by begin
+      unfold term.to_termctx,
+      unfold termctx.apply,
+      congr,
+      from ih₄,
+      from ih₅
+    end
+  end
+
+lemma unchanged_of_apply_propctx_without_hole {P: prop} {t: term}:
+      P.to_propctx t = P :=
+  begin
+    change (propctx.apply (prop.to_propctx P) t = P),
+    induction P,
+
+    case prop.term t₁ {
+      unfold prop.to_propctx,
+      unfold propctx.apply,
+      congr,
+      from unchanged_of_apply_termctx_without_hole
+    },
+
+    case prop.not P₁ ih {
+      unfold prop.to_propctx,
+      unfold propctx.apply,
+      congr,
+      from ih
+    },
+
+    case prop.and P₁ P₂ ih₁ ih₂ {
+      unfold prop.to_propctx,
+      change (propctx.apply (propctx.and (prop.to_propctx P₁) (prop.to_propctx P₂)) t = prop.and P₁ P₂),
+      unfold propctx.apply,
+      congr,
+      from ih₁,
+      from ih₂
+    },
+
+    case prop.or P₁ P₂ ih₁ ih₂ {
+      unfold prop.to_propctx,
+      change (propctx.apply (propctx.or (prop.to_propctx P₁) (prop.to_propctx P₂)) t = prop.or P₁ P₂),
+      unfold propctx.apply,
+      congr,
+      from ih₁,
+      from ih₂
+    },
+
+    case prop.pre t₁ t₂ {
+      unfold prop.to_propctx,
+      unfold propctx.apply,
+      congr,
+      from unchanged_of_apply_termctx_without_hole,
+      from unchanged_of_apply_termctx_without_hole
+    },
+
+    case prop.pre₁ op t₁ {
+      unfold prop.to_propctx,
+      unfold propctx.apply,
+      congr,
+      from unchanged_of_apply_termctx_without_hole
+    },
+
+    case prop.pre₂ op t₁ t₂ {
+      unfold prop.to_propctx,
+      unfold propctx.apply,
+      congr,
+      from unchanged_of_apply_termctx_without_hole,
+      from unchanged_of_apply_termctx_without_hole
+    },
+
+    case prop.post t₁ t₂ {
+      unfold prop.to_propctx,
+      unfold propctx.apply,
+      congr,
+      from unchanged_of_apply_termctx_without_hole,
+      from unchanged_of_apply_termctx_without_hole
+    },
+
+    case prop.call t₁ t₂ {
+      unfold prop.to_propctx,
+      unfold propctx.apply,
+      congr,
+      from unchanged_of_apply_termctx_without_hole,
+      from unchanged_of_apply_termctx_without_hole
+    },
+
+    case prop.forallc y t P₁ ih {
+      unfold prop.to_propctx,
+      unfold propctx.apply,
+      congr,
+      from unchanged_of_apply_termctx_without_hole,
+      from ih
+    },
+
+    case prop.exis y P₁ ih {
+      unfold prop.to_propctx,
+      unfold propctx.apply,
+      congr,
+      from ih
+    }
+  end
+
 -- call history to prop coercion
 
 def calls_to_prop: history → prop
